Checkpoint proof of monitorSession; now need to use alt select spec

new/proof/github_com/goose_lang/goose/testdata/examples/channel/etcd_session.v
@@ -14,7 +14,16 @@ Context {sem : go.Semantics} {package_sem : etcd_session.Assumptions}.
 Collection W := sem + package_sem.
 Set Default Proof Using "W".
 
-#[global] Instance : IsPkgInit (iProp Σ) etcd_session := define_is_pkg_init True%I.
+Definition is_inv : iProp Σ :=
+  "#Hmu" ∷ is_Mutex (global_addr etcd_session.mu) (
+      ∃ ch γch,
+        "sessionc" ∷ (global_addr etcd_session.sessionc) ↦{#1/2} ch ∗
+        "#Hsessionc" ∷ own_closeable_chan ch γch True closeable.Unknown ∗
+        "#Hsessionc_is" ∷ is_chan ch γch unit
+    )
+.
+
+#[global] Instance : IsPkgInit (iProp Σ) etcd_session := define_is_pkg_init is_inv%I.
 #[global] Instance : GetIsPkgInitWf (iProp Σ) etcd_session := build_get_is_pkg_init_wf.
 
 Lemma wp_initialize' get_is_pkg_init :
@@ -27,8 +36,8 @@ Proof.
   wp_apply (wp_package_init with "[$Hown] HΦ").
   { destruct Hinit as (-> & ?). reflexivity. }
   iIntros "Hown". wp_auto.
-  wp_apply wp_GlobalAlloc as "?".
-  wp_apply wp_GlobalAlloc as "?".
+  wp_apply wp_GlobalAlloc as "mu".
+  wp_apply wp_GlobalAlloc as "sessionc".
   wp_apply (primitive.wp_initialize' with "[$Hown]") as "(Hown & #?)".
   { naive_solver. }
   wp_apply (time.wp_initialize' with "[$Hown]") as "(Hown & #?)".
@@ -38,13 +47,16 @@ Proof.
   wp_apply (errors.wp_initialize' with "[$Hown]") as "(Hown & #?)".
   { naive_solver. }
 
-  wp_apply chan.wp_make1 as "* (? & % & ?)".
-  iEval (rewrite is_pkg_init_unfold /=). iFrame "∗#". done.
+  iApply wp_fupd.
+  wp_apply chan.wp_make1 as "* (#? & % & ?)".
+  iEval (rewrite is_pkg_init_unfold /=). iFrame "∗#".
+  iMod (alloc_closeable_chan with "[$] [$]") as "Hown".
+  iDestruct (own_closeable_chan_Unknown with "[$]") as "#?".
+  iDestruct "sessionc" as "[H ?]".
+  iMod (init_Mutex with "[$] [H]") as "#$".
+  { iFrame "∗#". }
+  done.
 Qed.
-
-Record etcd_session_names :=
-  {
-  }.
 
 Lemma wp_newSession :
   {{{ is_pkg_init etcd_session }}}
@@ -55,5 +67,63 @@ Proof.
   { wp_apply errors.wp_New as "% _". wp_end. }
   { wp_end. }
 Qed.
+
+Lemma wp_waitForSessionExpiration :
+  {{{ is_pkg_init etcd_session }}}
+    @! etcd_session.waitForSessionExpiration #()
+  {{{ RET #(); True }}}.
+Proof. wp_start. wp_end. Qed.
+
+Lemma wp_monitorSession ch γch :
+  {{{ is_pkg_init etcd_session ∗
+      "sessionc" ∷ (global_addr etcd_session.sessionc) ↦{#1/2} (ch : chan.t) ∗
+      "Hsessionc" ∷ own_closeable_chan ch γch True closeable.Open ∗
+      "#Hsessionc_is" ∷ is_chan ch γch unit
+  }}}
+    @! etcd_session.monitorSession #()
+  {{{ RET #(); True }}}.
+Proof.
+  wp_start as "@".
+  iAssert (
+      ∃ ch γch,
+  "sessionc" ∷ global_addr etcd_session.sessionc ↦{#1 / 2} ch ∗
+  "Hsessionc" ∷ (own_closeable_chan ch γch True closeable.Open ∨ own_closeable_chan ch γch True closeable.Closed)
+    )%I with "[sessionc Hsessionc]" as "HH".
+  { iFrame. }
+  wp_for "HH".
+  wp_apply wp_waitForSessionExpiration.
+  iDestruct (is_pkg_init_access with "[$]") as "#Hinv".
+  simpl. rewrite /is_inv. iNamed "Hinv".
+  wp_apply (wp_Mutex__Lock with "[]").
+  { iFrame "#". }
+  iIntros "[Hlocked Hown]". iNamedSuffix "Hown" "_inv".
+  wp_auto.
+  wp_bind.
+  iCombine "sessionc sessionc_inv" gives %Heq. subst.
+  iCombine "sessionc sessionc_inv" as "sessionc".
+  iApply (wp_wand _ _ _
+              (λ v,
+                 ⌜ v = execute_val ⌝ ∗
+                 ∃ ch γch,
+                   "sessionc" ∷ global_addr etcd_session.sessionc ↦ ch ∗
+                   "Hsessionc" ∷ own_closeable_chan ch γch True closeable.Open
+              )%I with "[sessionc Hsessionc]").
+  {
+    wp_apply chan.wp_select_nonblocking.
+    iSplit.
+    - rewrite big_andL_cons. iSplit.
+      + repeat iExists _; iSplitR; first done.
+        iFrame "#".
+        iApply blocking_rcv_implies_nonblocking.
+        iApply (closeable_chan_receive with "[$]").
+        iIntros "[_ #Hclosed]". wp_auto. iApply wp_fupd.
+        wp_apply chan.wp_make1 as "* (#? & % & ?)".
+        iMod (alloc_closeable_chan with "[$] [$]") as "Hown".
+        iDestruct (own_closeable_chan_Unknown with "[$]") as "#?".
+        iSplitR; first done. iFrame "∗#%". done.
+      + rewrite big_andL_nil //.
+    - wp_auto. iSplitR; first done. iFrame "∗#%". admit.
+    }
+Admitted.
 
 End wps.
